{{ % Localize command definitions

\chapter{Class 7}

For this chapter, we replace the word \emph{formula} in rules and 
proofs of a formal system by the word \emph{judgement}.

\section{Natural Deduction for Propositional Logic}

Judgements in Natural Deduction have the form $\Gamma \vdash \phi$, 
where $\Gamma$ is a set of formulas and $\varphi$ is a formula.
Semantically, for all interpretations $v$, if all formulas in 
$\Gamma$ are true in $v$, then $\phi$ is true in $v$.
Formal system for natural deduction defines a meta-symbol 
$\vdash_\text{meta}$ such that  $\vdash_\text{meta} (\Gamma \vdash 
\phi)$. 

\subsection{Judgements in Natural Deduction}

We use the notation $\Gamma, \phi$ to show $\Gamma \cup \{\phi\}$. 

\begin{enumerate}
  \item Axioms
  \[ \infer* [right=ax]
    { }{\Gamma, \phi \vdash \phi}
    \qquad\qquad \infer* [right=$\top$-intro]
    { }{\Gamma \vdash \top}
  \]
  
  \item False-elimination: if $\bot$ can be derived, then anything 
  can be derived.
  \[ \infer* [right=$\bot$-elim]
    {\Gamma \vdash \bot}{\Gamma \vdash \phi}
  \]

  \item And-elimination and -introduction
  \[ \infer* [right=$\land$-elim]
    {\Gamma \vdash \phi \land \psi}{\Gamma \vdash \phi}
    \qquad\qquad \infer* [right=$\land$-elim]
    {\Gamma \vdash \phi \land \psi}{\Gamma \vdash \psi}
    \qquad\qquad \infer* [right=$\land$-intro]
    {\Gamma \vdash \phi \\ \Gamma \vdash \psi}
    {\Gamma \vdash \phi \land \psi}
  \]

  \item Or-elimination and -introduction
  \[ \infer* [right=$\lor$-elim]
    {\Gamma \vdash \phi \lor \psi 
    \\ \Gamma, \phi \vdash \chi
    \\ \Gamma, \psi \vdash \chi}{\Gamma \vdash \chi}
    \qquad\qquad \infer* [right=$\lor$-intro]
    {\Gamma \vdash \phi}{\Gamma \vdash \phi \land \psi}
    \qquad \infer* [right=$\land$-intro]
    {\Gamma \vdash \phi}{\Gamma \vdash \psi \land \phi}
  \]

  \item Negation-elimination and -introduction
  \[ \infer* [right=$\neg$-elim]
    {\Gamma \vdash \phi \\ \Gamma \vdash \neg \phi}
    {\Gamma \vdash \bot}
    \qquad\qquad \infer* [right=$\neg$-intro]
    {\Gamma, \phi \vdash \bot}{\Gamma \vdash \neg \phi}
  \]
  \item Implication-elimination and -introduction
  \[ \infer* [right=$\rightarrow$-elim]
    {\Gamma \vdash \phi \\ \Gamma \vdash \phi \rightarrow \psi}
    {\Gamma \vdash \psi}
    \qquad\qquad \infer* [right=$\rightarrow$-intro]
    {\Gamma, \phi \vdash \psi}{\Gamma \vdash \phi \rightarrow \psi}
  \]
  Observe how $\rightarrow$-elim is similar to modus ponens.
\end{enumerate}

\begin{homework}
  Prove implication transitivity using Natural Deduction.
\end{homework}

\begin{example}
  Show $(\phi \rightarrow \psi) \rightarrow 
  (\neg \psi \rightarrow \neg \phi)$.
\end{example}
\begin{proof}
  \[ \infer* [right=$\rightarrow$-intro]
    { \infer* [right=$\rightarrow$-intro]
      { \infer* [right=$\neg$-intro]
        { \infer* [right=$\neg$-elim]
          { \phi \rightarrow \psi, \neg \psi, \phi \vdash \psi \\
            \phi \rightarrow \psi, \neg \psi, \phi \vdash \neg \psi
          }{\phi \rightarrow \psi, \neg \psi, \phi \vdash \bot}
        }{\phi \rightarrow \psi, \neg \psi \vdash \neg \phi}
      }{(\phi \rightarrow \psi) 
        \vdash (\neg \psi \rightarrow \neg \phi)}
    }{\vdash (\phi \rightarrow \psi) 
      \rightarrow (\neg \psi \rightarrow \neg \phi)}
  \]
  Now we have two goals to prove. 
  \[ \infer* [right=$\rightarrow$-elim]
    { \infer* [right=ax]
      { }{\phi \rightarrow \psi, \neg \psi, \phi \vdash \phi} \\
      \infer* [right=ax]
      { }{\phi \rightarrow \psi, \neg \psi, \phi 
          \vdash \phi \rightarrow \psi}
    }{\phi \rightarrow \psi, \neg \psi, \phi \vdash \psi}
    \qquad \infer* [right=ax]
      { }{\phi \rightarrow \psi, \neg \psi, \phi \vdash \neg \psi}
    \qquad 
  \]
\end{proof}
}} % End localization of command definitions
